\section{基本积分公式}

\begin{multicols}{2}
    \begin{spacing}{3}
        \noindent $\displaystyle \int{x^k}\mathrm{d}x = \frac{1}{k+1}x^{k+1} + C \quad k\neq1$

        \noindent $\displaystyle \int{\frac{1}{x^2}} = -\frac{1}{x} + C$

        \noindent $\displaystyle \int{\frac{1}{\sqrt{x}}} = 2\sqrt{x} + C$

        \noindent $\displaystyle \int{\frac{1}{x}} = \ln{\left| x \right|} + C$

        \noindent $\displaystyle \int{e^x}\mathrm{d}x = e^x + C$

        \noindent $\displaystyle \int{a^x}\mathrm{d}x = \frac{a^x}{\ln{a}} + C$

        \noindent $\displaystyle \int{\sin{x}}\mathrm{d}x = -\cos{x} + C$

        \noindent $\displaystyle \int{\cos{x}}\mathrm{d}x = \sin{x} + C$

        \noindent $\displaystyle \int{\tan{x}}\mathrm{d}x = -\ln{\left| \cos{x} \right|} + C$

        \noindent $\displaystyle \int{\cot{x}}\mathrm{d}x = \ln{\left| \sin{x} \right|} + C$

        \noindent $\displaystyle \int{\sec^2{x}}\mathrm{d}x = \tan{x} + C$

        \noindent $\displaystyle \int{\csc^2{x}}\mathrm{d}x = -\cot{x} + C$

        \noindent $\displaystyle \int{\sec{x}\tan{x}}\mathrm{d}x = \sec{x} + C$

        \noindent $\displaystyle \int{\csc{x}\cot{x}}\mathrm{d}x = -\csc{x} + C$

        \noindent $\displaystyle \int{\frac{1}{1 + x^2}}\mathrm{d}x = \arctan{x} + C$

        \noindent $\displaystyle \int{\frac{1}{a^2 + x^2}}\mathrm{d}x = \frac{1}{a}\arccot{\frac{x}{a}} + C$

        \noindent $\displaystyle \int{\frac{1}{\sqrt{1 - x^2}}}\mathrm{d}x = \arcsin{x} + C$

        \noindent $\displaystyle \int{\frac{1}{\sqrt{a^2 - x^2}}}\mathrm{d}x = \arcsin{\frac{x}{a}} + C$

        \noindent $\displaystyle \int{\sin^2{x}}\mathrm{d}x = \frac{x}{2} - \frac{\sin{2x}}{4} + C$

        \noindent $\displaystyle \int{\cos^2{x}}\mathrm{d}x = \frac{x}{2} + \frac{\sin{2x}}{4} + C$

        \noindent $\displaystyle \int{\tan^2{x}}\mathrm{d}x = \tan{x} - x + C$

        \noindent $\displaystyle \int{\cot^2{x}}\mathrm{d}x = - \cot{x} + x + C$

        \noindent $\displaystyle \int{u}\mathrm{d}v = uv - \int{v}\mathrm{d}u + C$

        \noindent $\displaystyle \int_{a}^{b}{f(x)}\mathrm{d}x = \int_{a}^{b}{f(a + b - x)}\mathrm{d}x$
    \end{spacing}
\end{multicols}

\begin{spacing}{3}
    \noindent $\displaystyle \int{\frac{\mathrm{d}x}{\cos{x}}} = \int{\sec{x}}\mathrm{d}x = \ln{\left| \sec{x} + \tan{x} \right| } + C$

    \noindent $\displaystyle \int{\frac{\mathrm{d}x}{\sin{x}}} = \int{\csc{x}}\mathrm{d}x = \ln{\left| \csc{x} - \cot{x} \right| } + C$

    \noindent $\displaystyle \int{\frac{1}{\sqrt{x^2 + a^2}}}\mathrm{d}x = \ln{(x + \sqrt{x^2 + a ^2})} + C$

    \noindent $\displaystyle \int{\frac{1}{\sqrt{x^2 - a^2}}}\mathrm{d}x = \ln{\left|x + \sqrt{x^2 - a ^2}\right|} + C$

    \noindent $\displaystyle \int{\frac{1}{x^2 - a^2}} \mathrm{d}x = \frac{1}{2a} \ln{\left| \frac{x - a}{x + a} \right|} + C$

    \noindent $\displaystyle \int{\frac{1}{a^2 - x^2}} \mathrm{d}x = \frac{1}{2a} \ln{\left| \frac{x + a}{x - a} \right|} + C$

    \noindent $\displaystyle \int{\sqrt{a^2 - x^2}}\mathrm{d}x = \frac{a^2}{2}\arcsin{\frac{x}{a}} + \frac{x}{2}\sqrt{a^2 - x^2} + C$

    \noindent $\displaystyle \int_{a}^{b}{f(x)}\mathrm{d}x = \frac{1}{2}\int_{a}^{b}{[f(x) + f(a + b - x)]}\mathrm{d}x$

    \noindent $\displaystyle \int_{a}^{b}{f(x)}\mathrm{d}x = \int_{a}^{\frac{a+b}{2}}{[f(x) + f(a + b - x)]}\mathrm{d}x$

    \noindent $\displaystyle \int_{0}^{\pi}{xf(\sin{x})}\mathrm{d}x = \frac{\pi}{2}\int_{0}^{\pi}{f(\sin{x})}\mathrm{d}x$

    \noindent $\displaystyle \int_{0}^{\pi}{xf(\sin{x})}\mathrm{d}x = \pi\int_{0}^{\frac{\pi}{2}}{f(\sin{x})}\mathrm{d}x$

    \noindent $\displaystyle \int_{0}^{\frac{\pi}{2}}{f(\sin{x})}\mathrm{d}x = \int_{0}^{\frac{\pi}{2}}{f(\cos{x})}\mathrm{d}x $

    \noindent $\displaystyle \int_{0}^{\frac{\pi}{2}}{f(\sin{x}, \cos{x})}\mathrm{d}x = \int_{0}^{\frac{\pi}{2}}{f(\sin{x}, \cos{x})}\mathrm{d}x $

    \noindent $\displaystyle \int_{a}^{b}{f(x)}\mathrm{d}x = \int_{-\frac{\pi}{2}}^{\frac{\pi}{2}}{f(\frac{a + b}{2} + \frac{b - a}{2}\sin{t}) \cdot \frac{b - a}{2}\cos{x}}\mathrm{d}x$

    \noindent $\displaystyle \int_{a}^{b}{f(x)}\mathrm{d}x = \int_{0}^{1}(b - a)f[a + (b - a)t]\mathrm{d}t$

    \noindent $\displaystyle \int_{-a}^{a}{f(x)}\mathrm{d}x = \int_{0}^{a}[f(x) + f(-x)]\mathrm{d}x (a > 0)$

    \noindent $\displaystyle \int_{0}^{\frac{\pi}{2}}{\sin^n{x}}\mathrm{d}x = \int_{0}^{\frac{\pi}{2}}{\sin^n{x}}\mathrm{d}x = \left\{ \begin{array}{l}
        \frac{n - 1}{n} \cdot \frac{n - 3}{n - 2} \cdot \cdots  \cdot \frac{2}{3} \cdot 1 \\
        \frac{n - 1}{n} \cdot \frac{n - 3}{n - 2} \cdot \cdots  \cdot \frac{1}{2} \cdot \frac{\pi}{2} \\
    \end{array}\right.$

    \noindent $\displaystyle \int_{0}^{\pi}{\sin^n{x}}\mathrm{d}x = \left\{ \begin{array}{l}
        2 \cdot \frac{n - 1}{n} \cdot \frac{n - 3}{n - 2} \cdots \frac{2}{3} \cdot 1 \\
        2 \cdot \frac{n - 1}{n} \cdot \frac{n - 3}{n - 2} \cdots \frac{2}{3} \cdot \frac{\pi}{2} \\
    \end{array}\right.$

    \noindent $\displaystyle \int_{0}^{\pi}{\cos^n{x}}\mathrm{d}x = \left\{ \begin{array}{l}
        0 \\
        2 \cdot \frac{n - 1}{n} \cdot \frac{n - 3}{n - 2} \cdots \frac{2}{3} \cdot \frac{\pi}{2}
    \end{array}\right.$

    \noindent $\displaystyle \int_{0}^{2\pi}{\sin^n{x}}\mathrm{d}x = \int_{0}^{2\pi}{\cos^n{x}}\mathrm{d}x =
        \left\{ \begin{array}{l}
        0 \\
        4 \cdot \frac{n - 1}{n} \cdot \frac{n - 3}{n - 2} \cdots \frac{2}{3} \cdot \frac{\pi}{2} \\
    \end{array}\right. $
\end{spacing}
