\section{泰勒及其展开式}

{
    \noindent 泰勒公式：

    $\displaystyle f(x) = f(x_0) + f'(x_0)(x-x_0) + \frac{f''(x_0)}{2} x^2$

    $\displaystyle \qquad \  + \cdots + \frac{f^{n}x_0}{n!} (x-x_0)^n + \frac{f^{n+1}(\theta)}{(n+1)!}(x - x_0)^{n+1}$
}


{
    \noindent 麦克劳林公式：

    $\displaystyle f(x) = f(0) + f'(0)x + \frac{f''(0)}{2} x^2 + \cdots +$

    $\displaystyle \qquad \ \frac{f^{n}(0)}{n!} x^n + \frac{f^{n+1}(\theta)}{(n+1)!}x^{n+1}$
}

\begin{multicols}{2}
    \begin{spacing}{\hangju}
        \noindent $e^x = 1 + x + \frac{1}{2!}x^2$

        \noindent $\ln{(1 + x)} = x - \frac{1}{2!}x^2$

        \noindent $\sin{x} = x - \frac{1}{3!}x^{3}$

        \noindent $\arcsin{x} = x + \frac{1}{3!}x^{3}$

        \noindent $\tan{x} = x + \frac{1}{3}x^3$

        \noindent $\arctan{x} = x - \frac{1}{3}x^3$

        \noindent $\cos{x} = 1 - \frac{1}{2!}x^2$

        \noindent $\frac{1}{1 - x} = 1 + x + x^2$

        \noindent $\frac{1}{1 + x} = 1 - x + x^2$

        \noindent $(1 + x)^\alpha = 1 + \alpha x + \frac{\alpha(\alpha - 1)}{2}x^2$
    \end{spacing}
\end{multicols}

